src/Fmajor.v
@@ -55,7 +55,7 @@ Definition env := PTree.t value.
 Inductive cont: Type :=
   | Kstop: cont                (**r stop program execution *)
   | Kseq: stmt -> cont -> cont          (**r execute stmt, then cont *)
-  (* | Kswitch : ident -> env -> cont -> cont  (**r env to return to when exiting switch *) *)
+  | Kreturn: expr -> cont -> cont (**r return the result of expr *)
   | Kcall: ident -> expr -> function -> env -> cont -> cont.
                                         (**r return to caller *)
 
@@ -66,11 +66,6 @@ Inductive state: Type :=
              (e: expr)                  (**r expression for return val *)
              (k: cont)                  (**r its continuation -- what to do next *)
              (e: env),                   (**r current local environment *)
-      state
-  | Callstate:                  (**r Invocation of a function *)
-      forall (f: fundef)                (**r function to invoke *)
-             (args: list value)           (**r arguments provided by caller *)
-             (k: cont),                  (**r what to do next  *)
       state
   | Returnstate:                (**r Return from a function *)
       forall (v: value)                   (**r Return value *)
@@ -114,7 +109,6 @@ End EVAL_EXPR.
 Fixpoint call_cont (k: cont) : cont :=
   match k with
   | Kseq s k => call_cont k
-  (* | Kswitch id e k => call_cont k  *)
   | _ => k
   end.
 
@@ -131,18 +125,14 @@ Fixpoint set_params (vl: list value) (il: list ident) {struct il} : env :=
   | _, _ => PTree.empty value
   end.
 
-(* Fixpoint bind_ids (ids : list ident) (vals : list value) (e : env) : env := *)
-(*   match ids,vals with *)
-(*   | id :: ids', v :: vs => bind_ids ids' vs (PTree.set id v e) *)
-(*   | _,_ => e *)
-(*   end. *)
-
 Fixpoint find_case (tag : Z) (cases : list (Z * stmt)) : option stmt :=
   match cases with
   | nil => None
   | (z,s) :: r =>
     if zeq tag z then Some s else find_case tag r
   end.
+
+Definition call_sig := mksignature (Tint::Tint::nil) (Some Tint) cc_default.
 
 Inductive step : state -> trace -> state -> Prop :=
   | step_assign: forall f lhs rhs exp k e v,
@@ -153,26 +143,24 @@ Inductive step : state -> trace -> state -> Prop :=
   | step_skip_seq: forall f s k e exp,
       step (State f Sskip exp (Kseq s k) e)
         E0 (State f s exp k e)
-  | step_skip_return: forall f k e v exp,
+  | step_skip_return: forall f k e v exp nonsense,
       is_call_cont k ->
       eval_expr e exp v ->
-      step (State f Sskip exp k e)
+      step (State f Sskip nonsense (Kreturn exp k) e)
            E0 (Returnstate v k)
   | step_call: forall f k (e : env) id efunc earg varg fname cargs fn exp bcode,
       eval_expr e earg varg -> (* the argument *)
       eval_expr e efunc (Close fname cargs) -> (* the function itself *)
       Genv.find_symbol ge fname = Some bcode ->
       Genv.find_funct_ptr ge bcode = Some fn ->
+      length fn.(fn_params) = 2%nat ->
+      fn.(fn_sig) = call_sig ->
       step (State f (Scall id efunc earg) exp k e) E0
-           (Callstate fn ((Close fname cargs) :: varg :: nil) (Kcall id exp f e k))
+           (State fn (fst fn.(fn_body)) (snd fn.(fn_body)) (Kreturn (snd fn.(fn_body)) (Kcall id exp f e k)) (set_params ((Close fname cargs) :: varg :: nil) fn.(fn_params)))
   | step_return: forall v f id e k exp,
       e ! id = None ->
       step (Returnstate v (Kcall id exp f e k))
         E0 (State f Sskip exp k (PTree.set id v e))
-  | step_into_function: forall f vargs k,
-      length vargs = length f.(fn_params) ->
-      step (Callstate f vargs k)
-        E0 (State f (fst f.(fn_body)) (snd f.(fn_body)) k (set_params vargs f.(fn_params)))
   | step_seq: forall f s1 s2 k exp e,
       step (State f (Sseq s1 s2) exp k e)
         E0 (State f s1 exp (Kseq s2 k) e)
@@ -194,10 +182,6 @@ Inductive step : state -> trace -> state -> Prop :=
       e ! targid = None ->
       step (State f (Sswitch targid cases target) exp k e)
         E0 (State f s exp k (PTree.set targid (Constr tag vargs) e)).
-  (* | step_switch_cont: forall f exp k e e' ansid v, *)
-  (*     eval_expr e' (Var ansid) v -> *)
-  (*     step (State f Sskip exp (Kswitch ansid e k) e') *)
-  (*       E0 (State f Sskip exp k (PTree.set ansid v e)). *)
 
 End RELSEM.
 
@@ -206,7 +190,8 @@ Inductive initial_state (p: program): state -> Prop :=
       let ge := Genv.globalenv p in
       Genv.find_symbol ge p.(prog_main) = Some b ->
       Genv.find_funct_ptr ge b = Some f ->
-      initial_state p (Callstate f nil Kstop).
+      let retexp := snd (fn_body f) in
+      initial_state p (State f (fst (fn_body f)) retexp (Kreturn retexp Kstop) (PTree.empty value)).
 
 Inductive final_state: state -> int -> Prop :=
   | final_state_intro: forall r v,
@@ -214,7 +199,6 @@ Inductive final_state: state -> int -> Prop :=
 
 Definition semantics (p: program) :=
   Semantics step (initial_state p) final_state (Genv.globalenv p).
-
 
 Lemma semantics_receptive:
   forall (p: program), receptive (semantics p).
